Congruence of substitution

Refinery/Ctx/Append.lean
@@ -1,4 +1,4 @@
-import Refinery.Ctx.Basic
+import Refinery.Ctx.SSplit
 
 namespace Refinery
 
@@ -9,22 +9,31 @@ def Ctx?.append (Γ Δ : Ctx? α) : Ctx? α := List.append Δ Γ
 instance Ctx?.instAppend : Append (Ctx? α) := ⟨Ctx?.append⟩
 
 @[simp]
-theorem Ctx?.append_nil (Γ : Ctx? α) : Γ.append .nil = Γ := rfl
+theorem Ctx?.append_nil (Γ : Ctx? α) : Γ ++ .nil = Γ := rfl
 
 @[simp]
-theorem Ctx?.nil_append (Δ : Ctx? α) : Ctx?.nil.append Δ = Δ := List.append_nil Δ
+theorem Ctx?.nil_append (Δ : Ctx? α) : Ctx?.nil ++ Δ = Δ := List.append_nil Δ
 
 @[simp]
 theorem Ctx?.append_cons (Γ Δ : Ctx? α) (v : Var? α)
-  : Γ.append (Δ.cons v) = (Γ.append Δ).cons v := rfl
+  : Γ ++ (Δ.cons v) = (Γ ++ Δ).cons v := rfl
 
 theorem Ctx?.append_assoc (Γ Δ Θ : Ctx? α)
-  : (Γ.append Δ).append Θ = Γ.append (Δ.append Θ) := (List.append_assoc Θ Δ Γ).symm
+  : (Γ ++ Δ) ++ Θ = Γ ++ (Δ ++ Θ) := (List.append_assoc Θ Δ Γ).symm
+
+def Ctx?.rev (Γ : Ctx? α) : Ctx? α := List.reverse Γ
+
+theorem Ctx?.rev_append (Γ Δ : Ctx? α)
+  : (Γ ++ Δ).rev = Δ.rev ++ Γ.rev := List.reverse_append
+
+@[simp] theorem Ctx?.rev_nil : Ctx?.nil.rev = Ctx?.nil (α := α) := rfl
+
+@[simp] theorem Ctx?.rev_rev (Γ : Ctx? α) : Γ.rev.rev = Γ := List.reverse_reverse Γ
 
 variable [HasQuant α]
 
 def Ctx?.Wk.append {Γ Γ' Δ Δ' : Ctx? α}
-  (ρΓ : Γ'.Wk Γ) (ρΔ : Δ'.Wk Δ) : (Γ'.append Δ').Wk (Γ.append Δ)
+  (ρΓ : Γ'.Wk Γ) (ρΔ : Δ'.Wk Δ) : (Γ' ++ Δ').Wk (Γ ++ Δ)
   := match ρΓ, ρΔ with
   | ρΓ, .nil => ρΓ
   | ρΓ, .cons ρΔ hvw => (ρΓ.append ρΔ).cons hvw
@@ -44,4 +53,27 @@ theorem Ctx?.Wk.append_skip
   {Γ Γ' Δ Δ' : Ctx? α} (ρΓ : Γ'.Wk Γ) (ρΔ : Δ'.Wk Δ) {v : Var? α} (hv : v.del)
   : ρΓ.append (ρΔ.skip hv) = (ρΓ.append ρΔ).skip hv := rfl
 
---TODO: nil_append, append_assoc, via cast
+def Ctx?.wkAppend (Γ Δ : Ctx? α) (v : Var? α) [hv : v.del]
+  : (Γ.cons v ++ Δ).Wk (Γ ++ Δ) := match Δ with
+  | .nil => Γ.wk0 v
+  | .cons Δ w => (Γ.wkAppend Δ v).scons w
+
+def Ctx?.SSplit.append {Γ Γl Γr Δ Δl Δr : Ctx? α}
+  (hΓ : Γ.SSplit Γl Γr) (hΔ : Δ.SSplit Δl Δr) : (Γ ++ Δ).SSplit (Γl ++ Δl) (Γr ++ Δr)
+  := match hΔ with
+  | .nil => hΓ
+  | .cons hΔ hvw => .cons (hΓ.append hΔ) hvw
+
+def Ctx?.At.append {Γ} (hΓ : Γ.At v n) (Δ : Ctx? α) [hΔ : Δ.del] : (Γ ++ Δ).At v (n + Δ.length)
+  := match Δ, hΔ with
+  | .nil, _ => hΓ
+  | .cons Δ _, hΔ => have _ := hΔ.tail; .there (hΓ.append Δ) hΔ.head
+
+def Ctx?.At.append' {Γ} (hΓ : Γ.At v n) (Δ : Ctx? α) [hΔ : Δ.del] : (Γ ++ Δ).At v (Δ.length + n)
+  := (hΓ.append Δ).cast rfl rfl (by rw [add_comm])
+
+def Ctx?.atAppend (Γ Δ : Ctx? α) [hΓ : Γ.del] [hΔ : Δ.del] (v w : Var? α) (h : v.Wk w)
+  : (Γ.cons v ++ Δ).At w Δ.length
+  := match Δ, hΔ with
+  | .nil, _ => .here hΓ h
+  | .cons Δ _, hΔ => have _ := hΔ.tail; .there (Γ.atAppend Δ v w h) hΔ.head
