Refinery/Ctx/Strengthen.lean
@@ -1,0 +1,10 @@
+import Refinery.Ctx.SSplit
+
+namespace Refinery
+
+variable {α : Type u}
+
+inductive Ctx?.Strn : Ctx? α → Ctx? α → Type _
+  | nil : Strn .nil .nil
+  | cons (v) : Strn Γ Δ → Strn (Γ.cons v) (Δ.cons v)
+  | zero (A) : Strn Γ Δ → Strn (Γ.cons ⟨A, 0⟩) Δ
