Refinery/Term/Extrinsic/Subst/OfWk.lean
@@ -1,0 +1,32 @@
+import Refinery.Term.Extrinsic.Subst.Effect
+
+namespace Refinery
+
+open HasQuant HasPQuant HasCommRel
+
+variable {φ : Type u} {α : Type v} {ε : Type w} [S : Signature φ α ε]
+
+def Term.Deriv?.wkOut
+  {Γ : Ctx? α} {a : Term φ (Ty α)} {v w : Var? α} (ρ : v.Wk w) (D : Γ ⊢? a : v) : (Γ ⊢? a : w) :=
+  match v, w, D, ρ with
+  | _, _, .valid _ _ _ _, _ => sorry
+  | ⟨A, 0⟩, ⟨_, 0⟩, .zero hΓ a _, _ => .zero hΓ a _
+
+
+def Term.Deriv?.bv0' (Γ : Ctx? α) {v w : Var? α} (ρ : v.Wk w) :
+  Γ.erase.cons v ⊢? .bv (φ := φ) 0 : w
+  := (Deriv?.bv0 Γ v).wkOut ρ
+
+def Term.SubstDS.lift' {Γ Δ : Ctx? α} (σ : SubstDS φ Γ Δ) {v w : Var? α} (ρ : v.Wk w)
+  : SubstDS φ (Γ.cons v) (Δ.cons w)
+  := .cons (a := .bv 0)
+           (.cons Γ.erase_right (.right _))
+           (σ.wkIn (Γ.wk0 v.erase))
+           sorry
+
+def Ctx?.Wk.toSubst {Γ Δ : Ctx? α} : Γ.Wk Δ → Term.SubstDS φ Γ Δ
+  | .nil => .nil inferInstance
+  | .cons ρ hvw => sorry
+  | .skip ρ hv => sorry
+
+namespace Term
