Refinery/Term/Extrinsic/Wf/DerivedRewrite.lean
@@ -369,6 +369,23 @@ theorem Eqv.let₂_pair_right {A B C D} {Γ Γc Γl Γm Γr : Ctx? α}
   induction a, b, c using quotInd₃
   exact Eqv.of_tm rfl
 
+theorem Eqv.let_pair_left_wk0 {A B C} {Γ Γc Γl Γm Γr : Ctx? α}
+  (hΓ : Γ.SSplit Γc Γr) (hΓc : Γc.SSplit Γl Γm)
+  (a : Eqv R Γr A) (b : Eqv R Γl B) (c : Eqv R (Γm.cons ⟨A, ⊤⟩) C)
+  (ea eb : ε) [ha : a.HasEff ea] [hb : b.HasEff eb] (he : ea ⇌ eb)
+  : a.let₁ hΓ (.pair (hΓc.cons (.right _)) (b.wk0 _) c)
+  = .pair (hΓ.s12_3_1_23 hΓc) b (.let₁ (hΓ.s12_3_23 hΓc) a c)
+  := by
+  rw [bind_pair]
+  conv => rhs; rw [bind_pair]
+  rw [
+    Ctx?.SSplit.comm, Var?.SSplit.comm,
+    let_comm (ea := ea) (eb := eb) (ha := ha) (hb := hb) (he := he),
+    wk0_let₁_right, let_let₁
+  ]
+  sorry
+
+
 -- theorem Eqv.let₂_pair_left_wk0_wk0 {A B C D} {Γ Γc Γl Γm Γr : Ctx? α}
 --   (hΓ : Γ.SSplit Γc Γr) (hΓc : Γc.SSplit Γl Γm)
 --   (a : Eqv R Γr (.tensor A B)) (b : Eqv R Γl C) (c : Eqv R ((Γm.cons ⟨A, ⊤⟩).cons ⟨B, ⊤⟩) D)
