Refinery/Term/Extrinsic/Wf/Pack.lean
@@ -1,0 +1,70 @@
+import Refinery.Term.Extrinsic.Wf.Wk
+import Refinery.Ctx.Append
+
+open HasQuant HasPQuant HasCommRel
+
+namespace Refinery
+
+variable {φ : Type u} {α : Type v}
+
+def Ctx?.rety (Γ : Ctx? α) : Ty α
+  := match Γ with
+  | .nil => .unit
+  | .cons Γ v => v.ety.tensor Γ.rety
+
+namespace Term
+
+variable {ε : Type w} [S : Signature φ α ε] {R : DRWS φ α}
+
+def Wf.ebv0 {Γ : Ctx? α} [hΓ : Γ.del] {v : Var? α} : Wf R (Γ.cons v) v.ety := match v with
+  | ⟨_, 0⟩ => .unit _
+  | ⟨_, (_ : Quant)⟩ => .bv0
+
+def Wf.pack : (Γ : Ctx? α) → Wf R Γ Γ.ety
+  | .nil => .unit .nil
+  | .cons Γ v => .pair Γ.erase_right.right ((pack Γ).wk0 v.erase) .ebv0
+
+def Eqv.ebv0 {Γ : Ctx? α} [hΓ : Γ.del] {v : Var? α} : Eqv R (Γ.cons v) v.ety := match v with
+  | ⟨_, 0⟩ => .unit _
+  | ⟨_, (_ : Quant)⟩ => .bv0
+
+theorem Eqv.ebv0_eq {Γ : Ctx? α} [hΓ : Γ.del] {v : Var? α}
+  : Eqv.ebv0 (R := R) (Γ := Γ) (v := v) = e⟦Wf.ebv0⟧ := by
+  cases v using Var?.casesZero <;> rfl
+
+variable [R.UWkCongr]
+
+def Eqv.pack : (Γ : Ctx? α) → Eqv R Γ Γ.ety
+  | .nil => .unit .nil
+  | .cons Γ v => .pair Γ.erase_right.right ((pack Γ).wk0 v.erase) .ebv0
+
+theorem Eqv.pack_eq {Γ : Ctx? α} : Eqv.pack (R := R) (Γ := Γ) = e⟦Wf.pack Γ⟧ := by
+  induction Γ <;> simp [Eqv.pack, Wf.pack, ebv0_eq, *] <;> rfl
+
+def Eqv.bvAppend (Γ Δ : Ctx? α) [hΓ : Γ.del] [hΔ : Δ.del] {A : Ty α} {q : Quant}
+  : Eqv R (Γ.cons ⟨A, q⟩ ++ Δ) A := Eqv.bv Δ.length (Γ.atAppend Δ _ _ (by simp))
+
+def Eqv.wkAppend {Γ Δ : Ctx? α} (a : Eqv R (Γ ++ Δ) A) (v : Var? α) [hv : v.del]
+  : Eqv R (Γ.cons v ++ Δ) A := a.wk (Γ.wkAppend Δ v)
+
+def Eqv.swapAppendQ {Γ Δ : Ctx? α} {q : Quant} (a : Eqv R ((Γ ++ Δ).cons ⟨A, q⟩) B)
+  : Eqv R (Γ.cons ⟨A, q⟩ ++ Δ) B
+  := .let₁ (Γ.erase_right.right.append Δ.erase_right)
+      (bvAppend _ _)
+      ((a.wkAppend (Δ := Δ.cons ⟨A, q⟩) ⟨A, 0⟩).pwk ((Ctx?.PWk.refl _).cons (by simp)))
+
+def Eqv.swapAppend {Γ Δ : Ctx? α} (a : Eqv R ((Γ ++ Δ).cons ⟨A, ⊤⟩) B)
+  : Eqv R (Γ.cons ⟨A, ⊤⟩ ++ Δ) B
+  := .let₁ (Γ.erase_right.right.append Δ.erase_right)
+      (bvAppend _ _) (a.wkAppend (Δ := Δ.cons ⟨A, ⊤⟩) ⟨A, 0⟩)
+
+-- def Eqv.revAppend {Γ Δ : Ctx? α} (a : Eqv R (Γ ++ Δ) A)
+--   : Eqv R (Γ ++ Δ.rev) A := match Δ with
+--   | .nil => a
+--   | .cons Δ v => (a.swapAppend (Γ := Γ) (Δ := Δ)).revAppend.castCtx sorry
+
+-- def Eqv.letPack {Γ Γl Γr Δ : Ctx? α}
+--   (hΓ : Γ.SSplit Γl Γr) (a : Eqv R Γr Δ.ety) (b : Eqv R (Γl ++ Δ) A) : Eqv R Γ A
+--   := match Δ with
+--   | .nil => sorry
+--   | .cons Δ v => .let₂ hΓ a sorry
