Refinery/Term/Syntax/Decompose.lean
@@ -1,0 +1,19 @@
+import Refinery.Term.Syntax.Basic
+
+namespace Refinery
+
+namespace Term
+
+variable {φ : Type u} {α : Type v}
+
+def subst0 (a : Term φ α) : Subst φ α | 0 => a | n + 1 => .bv n
+
+@[simp] theorem subst0_get_zero (a : Term φ α) : a.subst0.get 0 = a := rfl
+
+@[simp] theorem subst0_get_succ (a : Term φ α) (n : ℕ) : a.subst0.get (n + 1) = .bv n := rfl
+
+@[simp] theorem subst0_wk0 (a b : Term φ α) : (↑⁰ a).subst b.subst0 = a
+  := by rw [<-subst_renIn]; apply Term.subst_id
+
+theorem Subst.split (σ : Subst φ α) : σ = (σ.get 0).subst0 * (σ.renIn Nat.succ).lift := by
+  ext x; cases x <;> simp
